clean up unsound admit

theories/prob_eff_lang/probblaze/examples/unsound_bind.v
@@ -1,11 +1,10 @@
 From iris.proofmode Require Import base proofmode classes.
 From clutch.prob_eff_lang.probblaze Require Import logic proofmode spec_rules.
 
- Lemma rel_bind_unsound `{!probblazeRGS Σ}k1 k2 e1 e2 X Y R :
+ Definition rel_bind_unsound := ∀ `{!probblazeRGS Σ}k1 k2 e1 e2 X Y R,
    iThy_le X Y -∗
    REL e1 ≤ e2 <|X|> {{ (λ v1 v2, REL fill k1 v1 ≤ fill k2 v2 <|Y|> {{R}} )}} -∗
    REL fill k1 e1 ≤ fill k2 e2 <|Y|> {{R}}.
- Proof. Admitted.
 
  Section implementation.
 
@@ -31,7 +30,7 @@ From clutch.prob_eff_lang.probblaze Require Import logic proofmode spec_rules.
       ∃ p1 p2 : val, ⌜ e1 = do: op p1 ⌝%E ∗ ⌜ e2 = (do: op p2) ⌝%E ∗ Q #()%V #()%V)%I.
    Next Obligation. solve_proper. Qed.
    
-   Lemma unsound_bind :
+   Lemma unsound_bind (unsound : rel_bind_unsound) :
      ⊢ REL (handler1 op (handler2 op (do: op #1))) ≤ (handler1 op (handler2 op (do: op #2))) <|iThyBot|> {{ (λ v1 v2, ⌜v1 = v2⌝) }}.
    Proof.
      (* Uncomment the following to see why this lemma should fail *)
@@ -44,7 +43,7 @@ From clutch.prob_eff_lang.probblaze Require Import logic proofmode spec_rules.
        + iIntros (???) "(%&%&->&->&HQ) #Hkont //=".
          rel_pures_l; first set_solver.
          rel_pures_r; first set_solver. iPureIntro; done.
-     - iApply (rel_bind_unsound [HandleCtx _ _ _ _ _] [HandleCtx _ _ _ _ _]); first iApply iThy_le_refl.
+     - iApply (unsound _ _ [HandleCtx _ _ _ _ _] [HandleCtx _ _ _ _ _]); first iApply iThy_le_refl.
        iApply (rel_introduction _ _ (λ v1 v2, ⌜ v1 = #()%V ⌝ ∗ ⌜ v2 = #()%V ⌝)%I).
        + iExists #1, #2. repeat (iSplit; try iPureIntro; try done). 
        + iIntros "!# !> % % (-> & ->)". iApply rel_value. simpl.
@@ -52,4 +51,3 @@ From clutch.prob_eff_lang.probblaze Require Import logic proofmode spec_rules.
    Qed.
 
  End verification.
-       
